<?xml version="1.0"?>
<rdf:RDF xmlns="http://purl.org/aiaontology#"
		 xml:base="http://purl.org/aiaontology"
		 xmlns:rdf="http://www.w3.org/1999/02/22-rdf-syntax-ns#"
		 xmlns:owl="http://www.w3.org/2002/07/owl#"
		 xmlns:rdfs="http://www.w3.org/2000/01/rdf-schema#"
		 xmlns:xsd="http://www.w3.org/2001/XMLSchema#"
		 xmlns:aiao="http://purl.org/aiaontology#"
		 xmlns:lrml="http://docs.oasis-open.org/legalruleml/ns/v1.0/"
		 xmlns:prov="http://www.w3.org/ns/prov#"
		 xmlns:claimont="http://purl.org/claimont#"
		 xmlns:impactont="http://purl.org/impactont#"
		 xmlns:ruleml="http://www.ruleml.org/spec/"
		 xmlns:skos="http://www.w3.org/2004/02/skos/core#"
		 xmlns:terms="http://purl.org/dc/terms/"
		 xmlns:time="http://www.w3.org/2006/time#">
		 
  <owl:Ontology rdf:about="http://purl.org/aiaontology">
	<terms:title xml:lang="en">Anthropogenic Impact Accounting Ontology</terms:title>
	<terms:description xml:lang="en">An ontology for accounting for human impact on their environments. This ontology relies heavily on the 'claimont', 'impactont' and 'legalruleml' ontologies.</terms:description>
  </owl:Ontology>
  
  <!-- aiao:Agent class -->
  <owl:Class rdf:about="http://purl.org/aiaontology#Agent">
	<rdfs:subClassOf rdf:resource="http://docs.oasis-open.org/legalruleml/ns/v1.0/Agent"/>
	<owl:equivalentClass rdf:resource="http://www.w3.org/ns/prov#Agent"/>
<rdfs:comment>A thing that bears some form of accountability for the occurrence of another thing.</rdfs:comment>
<rdfs:comment>
  This class includes all kinds of human and human-comprised agents, such as natural persons, legal persons (e.g., companies) and cyber 
personas (e.g., User1234 on TalkSomeMore social media platform).

  AIAO strongly recommends distinguishing between different types of agents (such as those listed above), but will neither require nor 
prescribe such distinctions.
</rdfs:comment>
<rdfs:comment>An Agent may comprise other Agents.</rdfs:comment>
<skos:example xml:lang="en">natural person</skos:example>
<skos:example xml:lang="en">legal person</skos:example>
<skos:example xml:lang="en">company</skos:example>
<skos:example xml:lang="en">cyber persona</skos:example>
  </owl:Class>
  
  <!-- aiao:ImpactClaim class -->
  <owl:Class rdf:about="http://purl.org/aiaontology#ImpactClaim">
	<rdfs:subClassOf rdf:resource="http://purl.org/claimont#Claim"/>
	<rdfs:comment>A claim about the causal relation between an event and a state difference.</rdfs:comment>
  </owl:Class>
  
  <!-- aiao:StateClaim class -->
  <owl:Class rdf:about="http://purl.org/aiaontology#StateClaim">
	<rdfs:subClassOf rdf:resource="http://purl.org/claimont#Claim"/>
	<rdfs:comment>A claim about the state of a thing.</rdfs:comment>
  </owl:Class>
  
  <!-- aiao:Activity class -->
  <owl:Class rdf:about="http://purl.org/aiaontology#Activity">
	<rdfs:subClassOf rdf:resource="http://purl.org/impactont#Event"/>
	<rdfs:comment>An event that is orchestrated by an agent.</rdfs:comment>
	<rdfs:comment>A thing that an agent does, which impacts an environment.</rdfs:comment>
<rdfs:comment>
  Generating electricity, extracting minerals, protecting a forest, restoring a wetland, and transporting goods are all examples of activities.
</rdfs:comment>
<skos:example xml:lang="en">generating electricity</skos:example>
<skos:example xml:lang="en">extracting minerals</skos:example>
<skos:example xml:lang="en">protecting a forest</skos:example>
<skos:example xml:lang="en">restoring a wetland</skos:example>
<skos:example xml:lang="en">transporting goods</skos:example>
  </owl:Class>
  
  <owl:Class rdf:about="http://purl.org/aiaontology#AgentActivityRelation">
	<rdfs:comment>The relation between an agent and an activity, typically governed by a formal control (such as an employment contract).
</rdfs:comment>
  </owl:Class>
   
  <!-- aiao:Instrument class -->
  <owl:Class rdf:about="http://purl.org/aiaontology#Instrument">

<rdfs:comment>A thing used to perform an activity, but which is neither an input to the activity, nor an output of the activity.</rdfs:comment>
<rdfs:comment>A boiler, a truck and a turbine are all examples of instruments.</rdfs:comment>
<rdfs:comment>An Instrument may comprise other Instruments.</rdfs:comment>
<skos:example xml:lang="en">boiler</skos:example>
<skos:example xml:lang="en">truck</skos:example>
<skos:example xml:lang="en">turbine</skos:example>
  </owl:Class>
  
  <!-- aiao:NaturalProcess class -->
  <owl:Class rdf:about="http://purl.org/aiaontology#NaturalProcess">
	<rdfs:subClassOf rdf:resource="http://purl.org/impactont#Process"/>
	<rdfs:comment>A series of interrelated or interacting natural events without a primary human cause.</rdfs:comment>
  </owl:Class>
  
  <!-- aiao:Project class -->
  <owl:Class rdf:about="http://purl.org/aiaontology#Project">
	<rdfs:subClassOf rdf:resource="http://purl.org/impactont#Process"/>
	<rdfs:comment>A coordinated set of activities, subject to specific controls. The controls must include at least (a) an objective and (b) a limited duration.</rdfs:comment>
	<rdfs:comment>TODO: Create object predicates for the required controls.</rdfs:comment>
  </owl:Class>  
  
  <!-- aiao:Environment class -->
  <owl:Class rdf:about="http://purl.org/aiaontology#Environment">
	<rdfs:subClassOf rdf:resource="http://purl.org/impactont#Thing"/>
	<rdfs:comment>The surroundings and conditions in which a thing occurs.</rdfs:comment>

<rdfs:comment>
  This definition is not limited to physical or natural environments - social, political, economic, legal, etc. environments are also included.
</rdfs:comment>
<rdfs:comment>An Environment may comprise other Environments.</rdfs:comment>
<skos:example xml:lang="en">social environment</skos:example>
<skos:example xml:lang="en">political environment</skos:example>
<skos:example xml:lang="en">economic environment</skos:example>
<skos:example xml:lang="en">legal environment</skos:example>
<skos:example xml:lang="en">physical environment</skos:example>
<skos:example xml:lang="en">natural environment</skos:example>
  </owl:Class>
  
  <!-- aiao:Control class -->
  <owl:Class rdf:about="http://purl.org/aiaontology#Control">
	<owl:equivalentClass rdf:resource="http://www.ruleml.org/spec/Rule"/>

<rdfs:comment>A thing that limits or directs another thing.</rdfs:comment>
<rdfs:comment>
  A Control may comprise other Controls, e.g., a methodology (a Control) defines many conditions to be met (which are Controls themselves).
</rdfs:comment>
<rdfs:comment>The implementation plan and monitoring plan for an activity are controls.</rdfs:comment>
<skos:example xml:lang="en">implementation plan</skos:example>
<skos:example xml:lang="en">monitoring plan</skos:example>
<skos:example xml:lang="en">methodology</skos:example>

  </owl:Class>
  
  <!-- aiao:Objective class -->
  <owl:Class rdf:about="http://purl.org/aiaontology#Objective">
	<rdfs:subClassOf rdf:resource="http://purl.org/aiaontology#Control"/>
	<rdfs:comment>A desired state to be effected by an activity.</rdfs:comment>
	<skos:altLabel>Goal</skos:altLabel>
  </owl:Class>
  
  <!-- aiao:Role class -->
  <owl:Class rdf:about="http://purl.org/aiaontology#Role">
	<owl:equivalentClass rdf:resource="http://docs.oasis-open.org/legalruleml/ns/v1.0/Role"/>
	<rdfs:comment>A control that specifies the scope of and/or requirements for an agent's relation to an activity.</rdfs:comment>
	<rdfs:comment>
	  The extent to which an agent is accountable for the impact of an activity is determined by the role that they fulfil(led) in the activity.
	</rdfs:comment>

<rdfs:comment>
  Examples of roles include (but are not limited to) project developer, project owner, calibrator, operator, representer.
</rdfs:comment>
<skos:example xml:lang="en">project developer</skos:example>
<skos:example xml:lang="en">project owner</skos:example>
<skos:example xml:lang="en">calibrator</skos:example>
<skos:example xml:lang="en">operator</skos:example>
<skos:example xml:lang="en">representer</skos:example>

  </owl:Class>
  
  <!-- Disjoint Classes -->
  <owl:AllDisjointClasses>
<
  <owl:members rdf:parseType="Collection">
  <owl:Class rdf:about="#ImpactClaim"/>
  <owl:Class rdf:about="#StateClaim"/>
  </owl:members>
  </owl:AllDisjointClasses>  
  
  <owl:AllDisjointClasses>
  <owl:members rdf:parseType="Collection">
  <owl:Class rdf:about="#NaturalProcess"/>
  <owl:Class rdf:about="#Project"/>
  </owl:members>
  </owl:AllDisjointClasses>    
  
  <owl:ObjectProperty rdf:about="#hasObjective">
	  <rdfs:domain rdf:resource="#Activity"/>
	  <rdfs:domain rdf:resource="#Project"/>
	  <rdfs:range rdf:resource="#Objective"/>
  </owl:ObjectProperty>
  
	<owl:ObjectProperty rdf:ID="hasSubject">
    <rdfs:domain rdf:resource="#ImpactClaim"/>
    <rdfs:domain rdf:resource="#StateClaim"/>
    <rdfs:range rdf:resource="impactont:Impact"/>
    <rdfs:range rdf:resource="impactont:Thing"/>
</owl:ObjectProperty>
	
	<owl:ObjectProperty rdf:ID="hasAgentActivityRelation">
		<rdfs:domain rdf:resource="#Activity"/>
		<rdfs:domain rdf:resource="#Project"/>
		<rdfs:range rdf:resource="#AgentActivityRelation"/>
	</owl:ObjectProperty>

	<owl:ObjectProperty rdf:ID="governs">
		<owl:inverseOf rdf:resource="#isGovernedBy"/>
		<rdfs:domain rdf:resource="#Role"/>
		<rdfs:range rdf:resource="#AgentActivityRelation"/>
	</owl:ObjectProperty>

	<owl:ObjectProperty rdf:ID="hasAgent">
		<rdfs:domain rdf:resource="#AgentActivityRelation"/>
		<rdfs:range rdf:resource="#Agent"/>
	</owl:ObjectProperty>
	
	<owl:ObjectProperty rdf:ID="hasActivity">
		<rdfs:domain rdf:resource="#AgentActivityRelation"/>
		<rdfs:range rdf:resource="#Activity"/>
	</owl:ObjectProperty>	
  
	<owl:ObjectProperty rdf:ID="isPerformedWith">
		<rdfs:domain rdf:resource="#Activity"/>
		<rdfs:range rdf:resource="#Instrument"/>
	</owl:ObjectProperty>  
  
		<owl:ObjectProperty rdf:ID="comprisesActivity">
		<rdfs:domain rdf:resource="#Project"/>
		<rdfs:range rdf:resource="#Activity"/>
	</owl:ObjectProperty>    
  
	<owl:ObjectProperty rdf:ID="hasDuration">
		<rdfs:domain rdf:resource="#Project"/>
		<rdfs:range rdf:resource="time:Duration"/>
	</owl:ObjectProperty>     

</rdf:RDF>
