<?xml version="1.0"?>
<rdf:RDF xmlns="http://purl.org/aiaontology#"
		 xml:base="http://purl.org/aiaontology"
		 xmlns:rdf="http://www.w3.org/1999/02/22-rdf-syntax-ns#"
		 xmlns:owl="http://www.w3.org/2002/07/owl#"
		 xmlns:rdfs="http://www.w3.org/2000/01/rdf-schema#"
		 xmlns:xsd="http://www.w3.org/2001/XMLSchema#"
		 xmlns:aiao="http://purl.org/aiaontology#"
		 xmlns:lrml="http://docs.oasis-open.org/legalruleml/ns/v1.0/"
		 xmlns:prov="http://www.w3.org/ns/prov#"
		 xmlns:claimont="http://purl.org/claimont#"
		 xmlns:impactont="http://purl.org/impactont#"
		 xmlns:ruleml="http://www.ruleml.org/spec/"
		 xmlns:skos="http://www.w3.org/2004/02/skos/core#"
		 xmlns:terms="http://purl.org/dc/terms/">
		 
  <owl:Ontology rdf:about="http://purl.org/aiaontology">
	<terms:title xml:lang="en">Anthropogenic Impact Accounting Ontology</terms:title>
	<terms:description xml:lang="en">An ontology for accounting for human impact on their environments. This ontology relies heavily on the 'claimont', 'impactont' and 'legalruleml' ontologies.</terms:description>
  </owl:Ontology>
  
  <!-- aiao:Agent class -->
  <owl:Class rdf:about="http://purl.org/aiaontology#Agent">
	<rdfs:subClassOf rdf:resource="http://docs.oasis-open.org/legalruleml/ns/v1.0/Agent"/>
	<owl:equivalentClass rdf:resource="http://www.w3.org/ns/prov#Agent"/>
	<rdfs:comment>A thing that bears some form of accountability for the occurrence of another thing.</rdfs:comment>
	<rdfs:comment>
	  This class includes all kinds of human and human-comprised agents, such as natural persons, legal persons (e.g., companies) and cyber 
personas (e.g., User1234 on TalkSomeMore social media platform).

	  AIAO strongly recommends distinguishing between different types of agents (such as those listed above), but will neither require nor 
prescribe such distinctions.
	</rdfs:comment>
	<rdfs:comment>An Agent may comprise other Agents.</rdfs:comment>	
  </owl:Class>
  
  <!-- aiao:ImpactClaim class -->
  <owl:Class rdf:about="http://purl.org/aiaontology#ImpactClaim">
	<rdfs:subClassOf rdf:resource="http://purl.org/claimont#Claim"/>
	<rdfs:comment>A claim about the causal relation between an event and a state difference.</rdfs:comment>
  </owl:Class>
  
  <!-- aiao:StateClaim class -->
  <owl:Class rdf:about="http://purl.org/aiaontology#StateClaim">
	<rdfs:subClassOf rdf:resource="http://purl.org/claimont#Claim"/>
	<rdfs:comment>A claim about the state of a thing.</rdfs:comment>
  </owl:Class>
  
  <!-- aiao:Activity class -->
  <owl:Class rdf:about="http://purl.org/aiaontology#Activity">
	<rdfs:subClassOf rdf:resource="http://purl.org/impactont#Event"/>
	<rdfs:comment>An event that is orchestrated by an agent.</rdfs:comment>
	<rdfs:comment>A thing that an agent does, which impacts an environment.</rdfs:comment>
	<rdfs:comment>
	  Generating electricity, extracting minerals, protecting a forest, restoring a wetland, and transporting goods are all examples of activities.
	</rdfs:comment>
  </owl:Class>
  
  <owl:Class rdf:about="http://purl.org/aiaontology#AgentActivityRelation">
	<rdfs:comment>The relation between an agent and an activity, typically governed by a formal control (such as an employment contract).
</rdfs:comment>
  </owl:Class>
   
  <!-- aiao:Instrument class -->
  <owl:Class rdf:about="http://purl.org/aiaontology#Instrument">
	<rdfs:comment>A thing used to perform an activity, but which is neither an input to the activity, nor an output of the activity.</rdfs:comment>
	<rdfs:comment>A boiler, a truck and a turbine are all examples of instruments.</rdfs:comment>
	<rdfs:comment>An Instrument may comprise other Instruments.</rdfs:comment>
  </owl:Class>
  
  <!-- aiao:NaturalProcess class -->
  <owl:Class rdf:about="http://purl.org/aiaontology#NaturalProcess">
	<rdfs:subClassOf rdf:resource="http://purl.org/impactont#Process"/>
	<rdfs:comment>A series of interrelated or interacting natural events without a primary human cause.</rdfs:comment>
  </owl:Class>
  
  <!-- aiao:Project class -->
  <owl:Class rdf:about="http://purl.org/aiaontology#Project">
	<rdfs:subClassOf rdf:resource="http://purl.org/impactont#Process"/>
	<rdfs:comment>A coordinated set of activities, subject to specific controls. The controls must include at least (a) an objective and (b) a limited duration.</rdfs:comment>
	<rdfs:comment>TODO: Create object predicates for the required controls.</rdfs:comment>
  </owl:Class>  
  
  <!-- aiao:Environment class -->
  <owl:Class rdf:about="http://purl.org/aiaontology#Environment">
	<rdfs:subClassOf rdf:resource="http://purl.org/impactont#Thing"/>
	<rdfs:comment>The surroundings and conditions in which a thing occurs.</rdfs:comment>
	<rdfs:comment>
	  This definition is not limited to physical or natural environments - social, political, economic, legal, etc. environments are also included.
	</rdfs:comment>	
	<rdfs:comment>An Environment may comprise other Environments.</rdfs:comment>
  </owl:Class>
  
  <!-- aiao:Control class -->
  <owl:Class rdf:about="http://purl.org/aiaontology#Control">
	<owl:equivalentClass rdf:resource="http://www.ruleml.org/spec/Rule"/>
	<rdfs:comment>A thing that limits or directs another thing.</rdfs:comment>
	<rdfs:comment>
	  A Control may comprise other Controls, e.g., a methodology (a Control) defines many conditions to be met (which are Controls themselves).
	</rdfs:comment>
	<rdfs:comment>The implementation plan and monitoring plan for an activity are controls.</rdfs:comment>
  </owl:Class>
  
  <!-- aiao:Objective class -->
  <owl:Class rdf:about="http://purl.org/aiaontology#Objective">
	<rdfs:subClassOf rdf:resource="http://purl.org/aiaontology#Control"/>
	<rdfs:comment>A desired state to be effected by an activity.</rdfs:comment>
	<skos:altLabel>Goal</skos:altLabel>
  </owl:Class>
  
  <!-- aiao:Role class -->
  <owl:Class rdf:about="http://purl.org/aiaontology#Role">
	<owl:equivalentClass rdf:resource="http://docs.oasis-open.org/legalruleml/ns/v1.0/Role"/>
	<rdfs:comment>A control that specifies the scope of and/or requirements for an agent's relation to an activity.</rdfs:comment>
	<rdfs:comment>
	  The extent to which an agent is accountable for the impact of an activity is determined by the role that they fulfil(led) in the activity.
	</rdfs:comment>
	<rdfs:comment>
	  Examples of roles include (but are not limited to) project developer, project owner, calibrator, operator, representer.
	</rdfs:comment>
  </owl:Class>
  
  <!-- Disjoint Classes -->
  <owl:AllDisjointClasses>
	  <owl:members rdf:parseType="Collection">
		  <owl:Class rdf:about="#ImpactClaim"/>
		  <owl:Class rdf:about="#StateClaim"/>
	  </owl:members>
  </owl:AllDisjointClasses>	  
  
  <owl:AllDisjointClasses>
	  <owl:members rdf:parseType="Collection">
		  <owl:Class rdf:about="#NaturalProcess"/>
		  <owl:Class rdf:about="#Project"/>
	  </owl:members>
  </owl:AllDisjointClasses>	    
  
  <owl:ObjectProperty rdf:about="#hasObjective">
	  <rdfs:domain rdf:resource="#Activity"/>
	  <rdfs:domain rdf:resource="#Project"/>
	  <rdfs:range rdf:resource="#Objective"/>
  </owl:ObjectProperty>
  
	<owl:ObjectProperty rdf:ID="hasSubject">
		<rdfs:domain rdf:resource="#ImpactClaim"/>
		<rdfs:range rdf:resource="impactont:Impact"/>
	</owl:ObjectProperty>

	<owl:ObjectProperty rdf:ID="hasSubject">
		<rdfs:domain rdf:resource="#StateClaim"/>
		<rdfs:range rdf:resource="impactont:Thing"/>
	</owl:ObjectProperty>
	
	<owl:ObjectProperty rdf:ID="hasAgentActivityRelation">
		<rdfs:domain rdf:resource="#Activity"/>
		<rdfs:domain rdf:resource="#Project"/>
		<rdfs:range rdf:resource="#AgentActivityRelation"/>
	</owl:ObjectProperty>

	<owl:ObjectProperty rdf:ID="governs">
		<owl:inverseOf rdf:resource="#isGovernedBy"/>
		<rdfs:domain rdf:resource="#Role"/>
		<rdfs:range rdf:resource="#AgentActivityRelation"/>
	</owl:ObjectProperty>

	<owl:ObjectProperty rdf:ID="hasAgent">
		<rdfs:domain rdf:resource="#AgentActivityRelation"/>
		<rdfs:range rdf:resource="#Agent"/>
	</owl:ObjectProperty>
	
	<owl:ObjectProperty rdf:ID="hasActivity">
		<rdfs:domain rdf:resource="#AgentActivityRelation"/>
		<rdfs:range rdf:resource="#Activity"/>
	</owl:ObjectProperty>	
  
	<owl:ObjectProperty rdf:ID="isPerformedWith">
		<rdfs:domain rdf:resource="#Activity"/>
		<rdfs:range rdf:resource="#Instrument"/>
	</owl:ObjectProperty>  
  
		<owl:ObjectProperty rdf:ID="comprisesActivity">
		<rdfs:domain rdf:resource="#Project"/>
		<rdfs:range rdf:resource="#Activity"/>
	</owl:ObjectProperty>    
  
	<owl:ObjectProperty rdf:ID="hasDuration">
		<rdfs:domain rdf:resource="#Project"/>
		<rdfs:range rdf:resource="(TODO: A fixed temporal duration.)"/>
	</owl:ObjectProperty>     
	
	
	<!-- https://registry.goldstandard.org/projects/details/605 -->
	
	<owl:NamedIndividual rdf:ID="iofs(GS3492)drfysdf">
		<rdf:type rdf:resource="#Project"/>
		<comprisesActivity rdf:resource="GS3492Activity1"/>
		<comprisesActivity rdf:resource="GS3492Activity2"/>
		<comprisesActivity rdf:resource="GS3492Activity3"/>
		<hasObjective "Reduce the fuel consumption of ships through the application of advanced hull coatings."/>
		<hasDuration rdf:resource="(2013 - 2021)">
		<hasAgentActivityRelation rdf:resource="dfadbe8798df987adffa"/>
	</owl:NamedIndividual>
	
	<owl:NamedIndividual rdf:ID="GS3492Activity1">
		<rdf:type rdf:resource="#Activity"/>
		<hasObjective "Apply Intersleek 700 (only) to selected vessels."/>		
	</owl:NamedIndividual>

	<owl:NamedIndividual rdf:ID="GS3492Activity2">
		<rdf:type rdf:resource="#Activity"/>
		<hasObjective "Apply Intersleek 700 and Intersleek 1100SR to selected vessels."/>		
	</owl:NamedIndividual>

	<owl:NamedIndividual rdf:ID="GS3492Activity3">
		<rdf:type rdf:resource="#Activity"/>
		<hasObjective "Apply Intersleek 900 (only) to selected vessels."/>		
	</owl:NamedIndividual>	
	
	<owl:NamedIndividual rdf:ID="dsaf(InternationalPaintLtd)78df">
		<rdf:type rdf:resource="#Agent"/>
	</owl:NamedIndividual>		

	<owl:NamedIndividual rdf:ID="123a(ProjectOwnerOfAGoldStandardProject)f678">
		<rdf:type rdf:resource="#Role"/>
	</owl:NamedIndividual>	
	
	<owl:NamedIndividual rdf:ID="dfadbe8798df987adffa">
		<rdf:type rdf:resource="#AgentActivityRelation"/>
		<hasAgent rdf:resource="dsaf(InternationalPaintLtd)78df"/>
		<hasActivity rdf:resource="iofs(GS3492)drfysdf"/>
		<isGovernedBy rdf:resource="123a(ProjectOwnerOfAGoldStandardProject)f678"/>
	</owl:NamedIndividual>
	
	<owl:NamedIndividual rdf:ID="erte(CO2emissionsFromShipIndicator)ttre">
		<rdf:type rdf:resource="impactont:Indicator"/>
		<hasDefinition rdf:datatype="http://www.w3.org/2001/XMLSchema#string">The amount of carbon dioxide (CO2) emissions released per year by a maritime vessel due to the fuel consumption of its engines.</hasDefinition>
		<hasUnitOfMeasure rdf:datatype="http://www.w3.org/2001/XMLSchema#string">tCO2/yr</hasUnitOfMeasure>
	</owl:NamedIndividual>	
	
	
	

	<!--For each of the 17 ships involved in the project, the following individuals must be created:-->
	
	<owl:NamedIndividual rdf:ID="sadf(Ship9xxxx14/86366)aufy">
		<rdf:type rdf:resource="impactont:Thing"/>
	</owl:NamedIndividual>
	
	<owl:NamedIndividual rdf:ID="rfvf(VoyageLogForShip9xxxx14/86366)rfvf">
		<rdf:type rdf:resource="claimont:Substantiation"/>
	</owl:NamedIndividual>
	<!--A named individual like this must be created for each of the voyage logs of the ship.-->
	
	
	
	<owl:NamedIndividual rdf:ID="duifu(MonPer1BaselineStateForShip9xxxx14/86366)dfdf">
		<rdf:type rdf:resource="impactont:State"/>
		<impactont:hasTemporalLocation rdf:resource="(10 September 2014 - 9 September 2015)"/>
		<impactont:hasModality rdf:datatype="http://www.w3.org/2001/XMLSchema#string">counterfactual</hasModality>
		<impactont:isDefinedByIndicator rdf:resource="#erte(CO2emissionsFromShipIndicator)ttre">"/>
		<impactont:hasValue rdf:datatype="http://www.w3.org/2001/XMLSchema#decimal">119000</hasValue>		
	</owl:NamedIndividual>	
	<!--A named individual like this must be created for each monitoring period.-->	
	
	<owl:NamedIndividual rdf:ID="dudf(ClaimAboutMonPer1BaselineStateForShip9xxxx14/86366)qwqw">
		<rdf:type rdf:resource="#StateClaim"/>
		<claimont:hasClaimant rdf:resource="dsaf(InternationalPaintLtd)78df"/>
		<claimont:hasSubject rdf:resource="sadf(Ship9xxxx14/86366)aufy"/>
		<claimont:hasPredicate rdf:datatype="http://www.w3.org/2001/XMLSchema#string">Had baseline state during monitoring period 1 of GS3492Activity1</>
		<claimont:hasObject rdf:resource="duifu(MonPer1BaselineStateForShip9xxxx14/86366)dfdf"/>
		<claimont:isSupportedBy rdf:resource="rfvf(VoyageLogForShip9xxxx14/86366)rfvf"/>
	</owl:NamedIndividual>	
	<!--A named individual like this must be created for each monitoring period.-->
	
	
	
	<owl:NamedIndividual rdf:ID="yyifu(MonPer1ProjectStateForShip9xxxx14/86366)dfyy">
		<rdf:type rdf:resource="impactont:State"/>
		<impactont:hasTemporalLocation rdf:resource="(10 September 2014 - 9 September 2015)"/>
		<impactont:hasModality rdf:datatype="http://www.w3.org/2001/XMLSchema#string">real</hasModality>
		<impactont:isDefinedByIndicator rdf:resource="#erte(CO2emissionsFromShipIndicator)ttre">"/>
		<impactont:hasValue rdf:datatype="http://www.w3.org/2001/XMLSchema#decimal">101002</hasValue>		
	</owl:NamedIndividual>	  
	<!--A named individual like this must be created for each monitoring period.-->  
  
	<owl:NamedIndividual rdf:ID="dudf(ClaimAboutMonPer1ProjectStateForShip9xxxx14/86366)qwqw">
		<rdf:type rdf:resource="#StateClaim"/>
		<claimont:hasClaimant rdf:resource="dsaf(InternationalPaintLtd)78df"/>
		<claimont:hasSubject rdf:resource="sadf(Ship9xxxx14/86366)aufy"/>
		<claimont:hasPredicate rdf:datatype="http://www.w3.org/2001/XMLSchema#string">Had project state during monitoring period 1 of GS3492Activity1</>
		<claimont:hasObject rdf:resource="yyifu(MonPer1ProjectStateForShip9xxxx14/86366)dfyy"/>
		<claimont:isSupportedBy rdf:resource="rfvf(VoyageLogForShip9xxxx14/86366)rfvf"/>
	</owl:NamedIndividual>	  
	<!--A named individual like this must be created for each monitoring period.-->
  

  
	<owl:NamedIndividual rdf:ID="tyuc(StateDifferenceForShip9xxxx14/86366DuringMonPer1)tyuy">
        <rdf:type rdf:resource="impactont:Event"/>
		<impactont:hasStateA rdf:resource="duifu(MonPer1BaselineStateForShip9xxxx14/86366)dfdf"/>
		<impactont:hasStateB rdf:resource="yyifu(MonPer1ProjectStateForShip9xxxx14/86366)dfyy"/>
    </owl:NamedIndividual>	  
	<!--A named individual like this must be created for each monitoring period.-->
  
  	<owl:NamedIndividual rdf:ID="uuug(ClaimAboutImpactOfGS3492Activity1OnShip9xxxx14/86366DuringMonPer1)guuf">
		<rdf:type rdf:resource="#ImpactClaim"/>
		<claimont:hasClaimant rdf:resource="dsaf(InternationalPaintLtd)78df"/>
		<claimont:hasSubject rdf:resource="GS3492Activity1"/>
		<claimont:hasPredicate rdf:datatype="http://www.w3.org/2001/XMLSchema#string">caused</>
		<claimont:hasObject rdf:resource="tyuc(StateDifferenceForShip9xxxx14/86366DuringMonPer1)tyuy"/>
		<claimont:isSupportedBy rdf:resource="...(#TODO: project documentation)..."/>
	</owl:NamedIndividual>	
	<!--A named individual like this must be created for each monitoring period.-->



	<owl:NamedIndividual rdf:ID="tyuc(ImpactOfGS3492Activity1OnShip9xxxx14/86366)tyuy">
        <rdf:type rdf:resource="impactont:Impact"/>
		<impactont:hasStateA rdf:resource="duifu(MonPer1BaselineStateForShip9xxxx14/86366)dfdf"/>
		<impactont:hasStateB rdf:resource="yyifu(MonPer1ProjectStateForShip9xxxx14/86366)dfyy"/>
		<impactont:hasProvenance rdf:resource="GS3492Activity1"/>
    </owl:NamedIndividual>	
	<!--A named individual like this must be created for each monitoring period for each ship.-->
 
  
</rdf:RDF>
